rocq-osiris/theories/stdlib/proofs/array.v
@@ -1,24 +1,148 @@
-From osiris.lang Require Import type_nel encode.
+From osiris.lang Require Import type_nel encode notations int.
 From osiris.program_logic Require Import program_logic.
 From osiris.proofmode Require Import proofmode.
 
-From osiris.stdlib Require Import og_array.
+From osiris.stdlib Require Import translated_array.
+
+From iris Require Import ltac_tactics.
+
+From osiris.logic Require Import list_z.
 
 Section proof.
 
   Context `{!osirisGS Σ}.
 
-  Definition invert_spec : Z → val → microvx → iProp Σ :=
+  Open Scope Z.
+
+  Definition init_spec : Z → val → microvx → iProp Σ :=
     λ n f m,
-      (∀ `(_ : Encode A) Φ,
-         iSpec τ[Z] f Φ -∗
-         imp m {{ λ a, isArray a n ∗ ∃ (xs : list A), isSlice (DfracOwn 1) a n xs }})%I.
+      (∀ `(_ : Encode A) `(_ : Inhabited A) (Φ : Z → A → iProp Σ) ,
+         ⌜0 ≤ n ≤ max_array⌝ -∗
+         □ iSpec τ[Z] f (λ i m, imp m {{ Φ i }}) -∗
+         imp m {{ λ a, ∃ (xs : list A), ⌜length xs = n⌝ ∗ ownArray a xs ∗
+                                     [∗ list] i↦x ∈ xs, Φ i x }})%I.
 
   Definition init := (EAnonFun __fun8).
 
-  Lemma ewp_invert η :
-    ⊢ imp (eval η init) {{ λ c, □ iSpec τ[Z; val] c invert_spec }}.
+  Lemma imp_init η :
+    ⊢ imp (eval η init) {{ λ c, □ iSpec τ[Z; val] c init_spec }}.
   Proof.
-  Admitted.
+    iApply imp_EAnon_pers.
+    iIntros "!> /=".
+    iIntros (n f).
+    change (VInt (int.repr n)) with #n.
+    unfold init_spec.
+    iIntros (A HencA HinhA Φ) "%Hbounds #Hf".
+    iApply imp_please; iNext.
+    iApply imp_EIfThenElse.
+    { iApply (imp_EOpEq_Z _ _ _ n 0). representable. representable.
+      - iApply imp_EPath. iApply imp_ret; auto.
+      - iApply imp_EInt. }
+    iIntros ([|]) "%Heq0".
+
+    { (* Case: [n = 0]. *)
+      iApply imp_mono_ret.
+      iApply (imp_EArrayLit (A:=A) []).
+      - iPureIntro; split; [ reflexivity | ].
+        rewrite length_nil. lia.
+      - simpl_evals. iApply (imp_ret [] []). reflexivity.
+        done.
+      - iIntros (a) "(%xs & Harray & Hemp)".
+        iPoseProof (big_sepL2_length with "Hemp") as "%Hlen".
+        apply list.nil_length_inv in Hlen as ->.
+        iFrame. rewrite length_nil. iSplit; [ iPureIntro; lia | auto ]. }
+
+    iApply imp_EIfThenElse.
+    { iApply (imp_EOpLt_Z _ _ _ n 0). representable. representable.
+      - iApply imp_EPath. iApply imp_ret; auto.
+      - iApply imp_EInt. }
+    iIntros ([|]) "%Hlt0".
+
+    { (* Case: [n < 0]. *)
+      (* This case is forbidden by the spec. *) lia. }
+
+    iApply (imp_ELet_var (B:=array)).
+    { (* Subgoal: [make l (f 0)] *)
+      iApply (imp_EArrayMake (A:=A) n). iPureIntro; assumption.
+      iApply imp_EPath. iApply imp_ret; eauto.
+      { iApply (imp_EApp τ[Z]).
+        iApply imp_EPath. iApply imp_ret; auto.
+        iApply imp_EInt.
+        iIntros (?) "-> %m $". } }
+    iIntros (res) "(%x & HΦx & #Harr & Hslice)".
+
+    (* Subgoal: [for i = 1 to ... done; res]. *)
+    iApply (imp_ESeq with "[Hslice HΦx]").
+
+    { (* Subgoal: [for i = 1 to ... done]. *)
+      iApply (imp_EFor
+                (λ i,
+                   isSlice (DfracOwn 1) res i (replicate (n - i) x) ∗
+                   ∃ xs, ⌜length xs = i⌝ ∗ isSlice (DfracOwn 1) res 0 xs ∗
+                            [∗ list] j↦x ∈ take i xs, Φ j x)%I
+                1 (n-1) with "[] [] [Hslice HΦx]").
+      representable. representable.
+      { iApply imp_EInt. }
+      { iApply (imp_EIntSub).
+        - instantiate (1:=(λ i,⌜i=n⌝)%I). iApply imp_EPath. iApply imp_ret; auto.
+        - iApply imp_EInt.
+        - iIntros "!> %% -> ->". auto. }
+      { rewrite unroll_replicate; last lia.
+        rewrite cons_is_append.
+        iPoseProof (split_Slice 1 with "Hslice") as "[Hslice1 Hslice2]".
+        reflexivity. done. iFrame. auto. }
+
+      iIntros "!>" (i' Hbound) "(Hslice1 & %xs & %Hlenxs & Hslice2 & HΦs)".
+      iApply (imp_EArraySet2 (A:=A)).
+      { iApply imp_EPath.
+        instantiate (1:=(λ a', ⌜a'=res⌝)%I).
+        iApply imp_ret; auto. }
+      { iApply imp_EPath.
+        instantiate (1:=(λ i, ⌜i = i'⌝)%I).
+        iApply imp_ret; auto. }
+      { iApply (imp_EApp τ[Z]).
+        iApply imp_EPath. iApply imp_ret; auto.
+        iApply imp_EPath.
+        instantiate (1:=(λ i, ⌜i = i'⌝)%I).
+        iApply imp_ret; auto.
+        iIntros "% -> % $". }
+
+      iIntros (?? y) "-> -> HΦ".
+      iFrame "#".
+      iCombine "Hslice2 Hslice1" as "Hslice".
+      iPoseProof (split_Slice with "Hslice") as "Hslice".
+      reflexivity. lia.
+
+      iFrame.
+      iSplit; iNext.
+      - iPureIntro. rewrite length_app length_replicate.
+        lia.
+      - iIntros "Hslice".
+        iPoseProof (split_Slice (i'+1) _ _ _ _ (xs ++ [y]) with "Hslice")
+          as "[Hslice0 Hslicei]".
+        { rewrite unroll_replicate; last lia.
+          rewrite cons_is_append. rewrite app_assoc.
+          rewrite insert_app_l; last (rewrite length_app length_singleton; lia).
+          rewrite insert_app_r; last lia.
+          rewrite insert_singleton. case_decide; last lia.
+          reflexivity. }
+        { rewrite length_app length_singleton. lia. }
+        replace (n - (i' + 1)) with (n - i' -1) by lia.
+        iFrame.
+        iSplit; first (iPureIntro; rewrite length_app length_singleton; lia).
+        take.
+        rewrite big_sepL_snoc. iFrame.
+        rewrite /length in Hlenxs. rewrite Hlenxs.
+        iApply "HΦ". }
+
+    iIntros "(Hslempty & %xs & %Hlen & Hslice & HΦs)".
+    iApply imp_EPath. iApply imp_ret; first encode.
+    take.
+    iFrame. rewrite length_replicate. rewrite Hlen.
+    replace (n - 1 + 1) with n by lia.
+    assert (n `max` 0 = n) as -> by lia.
+    assert (n `max` 1 = n) as -> by lia.
+    by iFrame "#".
+  Qed.
 
 End proof.
